misc

thys/lib/MM/Generic_Memory.thy
@@ -1,70 +1,8 @@
+section \<open>Memory Model\<close>
 theory Generic_Memory
 imports NEMonad
 begin
-
-  datatype 'v cell = FRESH | FREED | is_block: BLOCK (vals: "'v list")
-  hide_const (open) is_block vals
-
-  datatype addr = ADDR (block: nat) (index: int) 
-  hide_const (open) block index
-  
-  class infinite =
-    assumes infinite_UNIV[simp,intro!]: "\<not> finite (UNIV :: 'a set)"
-
-  instance nat :: infinite  
-    apply standard
-    by simp
-      
-  type_synonym block = nat  
-    
-  typedef 'v memory = "{ f :: block \<Rightarrow> 'v cell . finite {a. f a \<noteq> FRESH} }" 
-    by (auto intro: exI[where x="\<lambda>_. FRESH"])
-
-  setup_lifting type_definition_memory  
-
-  lift_definition mapp :: "'v memory \<Rightarrow> block \<Rightarrow> 'v cell" is "\<lambda>m a. m a" .
-  lift_definition mmap :: "'v memory \<Rightarrow> block \<Rightarrow> ('v cell \<Rightarrow> 'v cell) \<Rightarrow> 'v memory" is "\<lambda>m a f. m(a := f (m a))"
-  proof goal_cases
-    case (1 f a fx)
-    thm 1
-    have "{aa. (f(a := cell)) aa \<noteq> FRESH} \<subseteq> insert a {a. f a \<noteq> FRESH}" for cell
-      by auto
-    moreover from 1 have "finite \<dots>" by auto
-    ultimately show ?case by (meson finite_subset)
-  qed
-    
-  lemma mapp_mmap[simp]: "mapp (mmap f a g) = (mapp f)(a:=g (mapp f a))"
-    apply transfer
-    by auto
-
-  lemma mext: "f=f' \<longleftrightarrow> (\<forall>a. mapp f a = mapp f' a)"
-    apply transfer
-    by auto
-
-  definition "block_size m b \<equiv> case mapp m b of 
-    BLOCK vs \<Rightarrow> length vs
-  | _ \<Rightarrow> 0"
-
-  abbreviation "is_FRESH m b \<equiv> mapp m b = FRESH"  
-  abbreviation "is_ALLOC m b \<equiv> cell.is_block (mapp m b)"  
-  abbreviation "is_FREED m b \<equiv> mapp m b = FREED"  
-
-  lemma block_size_noblock[simp]:
-    "is_FRESH m b \<Longrightarrow> block_size m b = 0"
-    "is_FREED m b \<Longrightarrow> block_size m b = 0"
-    "\<not>is_ALLOC m b \<Longrightarrow> block_size m b = 0"
-    by (auto simp: block_size_def split: cell.splits)
-    
-  lemma is_ALLOC_conv: "is_ALLOC s b \<longleftrightarrow> \<not>is_FREED s b \<and> \<not>is_FRESH s b"  
-    apply auto
-    using cell.exhaust_disc by blast
-    
-  lemma is_block_state_simps: 
-    "is_FREED s b \<Longrightarrow> \<not>is_ALLOC s b \<and> \<not>is_FRESH s b"
-    "is_FRESH s b \<Longrightarrow> \<not>is_ALLOC s b \<and> \<not>is_FREED s b"
-    by (auto)
-      
-    
+  subsection \<open>Miscellaneous\<close>
   definition "i_nth xs i \<equiv> if i\<in>{0..<int (length xs)} then xs!nat i else undefined"  
   definition "i_upd xs i x \<equiv> if i\<in>{0..<int (length xs)} then xs[nat i:=x] else xs"
         
@@ -88,54 +26,151 @@ begin
     "i\<noteq>j \<Longrightarrow> i_nth (i_upd xs i x) j = i_nth xs j"
     by (auto simp: i_upd_def i_nth_def)
     
+
+  definition list_combine where
+    "list_combine xs\<^sub>1 I xs\<^sub>2 \<equiv> map (\<lambda>i. if i\<in>I then xs\<^sub>2!i else xs\<^sub>1!i) [0..<length xs\<^sub>1 ]"
+    
+  lemma nth_undefined: "\<not>i<length xs \<Longrightarrow> xs!i = undefined (i-length xs)"
+    apply (induction xs arbitrary: i)
+    apply (simp add: nth_def)
+    by auto
+    
+  lemma list_combine_nth: "length xs\<^sub>1 = length xs\<^sub>2 \<Longrightarrow> list_combine xs\<^sub>1 I xs\<^sub>2 ! i = (if i\<in>I then xs\<^sub>2!i else xs\<^sub>1!i)"  
+    unfolding list_combine_def
+    apply (cases "i<length xs\<^sub>2")
+    subgoal by (auto simp: )
+    subgoal by (simp add: nth_undefined)
+    done
+
+  lemma list_combine_length[simp]: "length (list_combine xs\<^sub>1 I xs\<^sub>2) = length xs\<^sub>1"  
+    by (auto simp: list_combine_def)
+    
+  lemma list_combine_inth: "length xs\<^sub>1 = length xs\<^sub>2 \<Longrightarrow> i_nth (list_combine xs\<^sub>1 I xs\<^sub>2) i = (if nat i\<in>I then i_nth xs\<^sub>2 i else i_nth xs\<^sub>1 i)"  
+    apply (cases "0\<le>i"; simp)
+    apply (cases "nat i < length xs\<^sub>1"; auto simp: list_combine_nth)
+    done
+    
+
+  subsection \<open>Memory Type Definition\<close>
+  text \<open>We define the memory model abstracted over the value type first.
+    Only later, we instantiate the value type with LLVM specific values
+  \<close>
+  
+  datatype 'v block = FRESH | FREED | is_alloc: ALLOC (vals: "'v list")
+  hide_const (open) is_alloc vals
+
+  text \<open>For technical reasons, we use integers as indexes. These are, however, always positive.\<close>
+  datatype addr = ADDR (block: nat) (index: int) 
+  hide_const (open) block index
+  
+  class infinite =
+    assumes infinite_UNIV[simp,intro!]: "\<not> finite (UNIV :: 'a set)"
+
+  instance nat :: infinite  
+    apply standard
+    by simp
+      
+  type_synonym block_idx = nat  
+    
+  typedef 'v memory = "{ f :: block_idx \<Rightarrow> 'v block . finite {a. f a \<noteq> FRESH} }" 
+    by (auto intro: exI[where x="\<lambda>_. FRESH"])
+
+  setup_lifting type_definition_memory  
+
+  text \<open>We define a get (mapp) and map (mmap) function for blocks of memory. 
+    These will be used as the only interface to the memory type from now on.\<close>
+  
+  lift_definition mapp :: "'v memory \<Rightarrow> block_idx \<Rightarrow> 'v block" is "\<lambda>m a. m a" .
+  lift_definition mmap :: "'v memory \<Rightarrow> block_idx \<Rightarrow> ('v block \<Rightarrow> 'v block) \<Rightarrow> 'v memory" is "\<lambda>m a f. m(a := f (m a))"
+  proof goal_cases
+    case (1 f a fx)
+    thm 1
+    have "{aa. (f(a := block)) aa \<noteq> FRESH} \<subseteq> insert a {a. f a \<noteq> FRESH}" for block
+      by auto
+    moreover from 1 have "finite \<dots>" by auto
+    ultimately show ?case by (meson finite_subset)
+  qed
+    
+  lemma mapp_mmap[simp]: "mapp (mmap f a g) = (mapp f)(a:=g (mapp f a))"
+    apply transfer
+    by auto
+
+  lemma mext: "f=f' \<longleftrightarrow> (\<forall>a. mapp f a = mapp f' a)"
+    apply transfer
+    by auto
+
+  subsection \<open>Block State\<close>  
+    
+  definition "block_size m b \<equiv> case mapp m b of 
+    ALLOC vs \<Rightarrow> length vs
+  | _ \<Rightarrow> 0"
+
+  abbreviation "is_FRESH m b \<equiv> mapp m b = FRESH"  
+  abbreviation "is_ALLOC m b \<equiv> block.is_alloc (mapp m b)"  
+  abbreviation "is_FREED m b \<equiv> mapp m b = FREED"  
+
+  lemma block_size_noblock[simp]:
+    "is_FRESH m b \<Longrightarrow> block_size m b = 0"
+    "is_FREED m b \<Longrightarrow> block_size m b = 0"
+    "\<not>is_ALLOC m b \<Longrightarrow> block_size m b = 0"
+    by (auto simp: block_size_def split: block.splits)
+    
+  lemma is_ALLOC_conv: "is_ALLOC s b \<longleftrightarrow> \<not>is_FREED s b \<and> \<not>is_FRESH s b"  
+    apply auto
+    using block.exhaust_disc by blast
+    
+  lemma is_block_state_simps: 
+    "is_FREED s b \<Longrightarrow> \<not>is_ALLOC s b \<and> \<not>is_FRESH s b"
+    "is_FRESH s b \<Longrightarrow> \<not>is_ALLOC s b \<and> \<not>is_FREED s b"
+    by (auto)
+      
+  subsection \<open>Accessing Memory via Addresses\<close>  
     
   definition "get_addr m a \<equiv> 
-    case a of ADDR b i \<Rightarrow> i_nth (cell.vals (mapp m b)) i
+    case a of ADDR b i \<Rightarrow> i_nth (block.vals (mapp m b)) i
   "  
     
   text \<open>The \<open>put\<close> function is closed to do nothing on invalid addresses. 
     This removes a lot of side-conditions from the lens laws below, 
     making them simpler to reason with.\<close>
   definition "put_addr m a x \<equiv> 
-    case a of ADDR b i \<Rightarrow> mmap m b (\<lambda>BLOCK vs \<Rightarrow> BLOCK (i_upd vs i x) | c \<Rightarrow> c )
+    case a of ADDR b i \<Rightarrow> mmap m b (\<lambda>ALLOC vs \<Rightarrow> ALLOC (i_upd vs i x) | c \<Rightarrow> c )
   "
 
   lemma block_size_put[simp]:
     "block_size (put_addr m a x) b = block_size m b"
     unfolding block_size_def put_addr_def 
-    by (auto split: addr.splits cell.splits simp: mext)
+    by (auto split: addr.splits block.splits simp: mext)
   
   lemma addr_put_get[simp]: "put_addr m a (get_addr m a) = m"
     and addr_put_put[simp]: "put_addr (put_addr m a y) a x = put_addr m a x"
     unfolding get_addr_def put_addr_def 
-    by (auto split: addr.splits cell.splits simp: mext)
+    by (auto split: addr.splits block.splits simp: mext)
     
     
   definition "is_valid_addr m a \<equiv> 
     case a of ADDR b i \<Rightarrow> 0\<le>i \<and> nat i < block_size m b"  
     
   lemma is_valid_addr_alt: "is_valid_addr m a = (case a of ADDR b i \<Rightarrow> is_ALLOC m b \<and> 0\<le>i \<and> nat i < block_size m b)"  
-    by (auto simp: is_valid_addr_def block_size_def split: addr.splits cell.split)
+    by (auto simp: is_valid_addr_def block_size_def split: addr.splits block.split)
 
   definition "is_valid_ptr_addr m a \<equiv> 
     case a of ADDR b i \<Rightarrow> is_ALLOC m b \<and> 0\<le>i \<and> nat i \<le> block_size m b"  
     
           
+  text \<open>Lens laws\<close>  
   lemma addr_get_put[simp]: "is_valid_addr m a \<Longrightarrow> get_addr (put_addr m a x) a = x"
     and addr_put_valid[simp]: "is_valid_addr (put_addr m a x) a' \<longleftrightarrow> is_valid_addr m a'"
     and addr_put_ptr_valid[simp]: "is_valid_ptr_addr (put_addr m a x) a' \<longleftrightarrow> is_valid_ptr_addr m a'"
     unfolding is_valid_addr_def is_valid_ptr_addr_def block_size_def get_addr_def put_addr_def
-    by (auto split: addr.splits cell.splits)
-    
-  lemma nat_nat_eq_conv: "nat i = nat i' \<longleftrightarrow> (i\<le>0 \<and> i'\<le>0) \<or> i=i'"  
-    by auto
+    by (auto split: addr.splits block.splits)
     
   lemma addr_indep[simp]: "\<lbrakk> is_valid_addr m a\<^sub>1; is_valid_addr m a\<^sub>2; a\<^sub>1\<noteq>a\<^sub>2\<rbrakk> \<Longrightarrow> get_addr (put_addr m a\<^sub>1 x) a\<^sub>2 = get_addr m a\<^sub>2"    
     unfolding is_valid_addr_def get_addr_def put_addr_def 
-    by (auto split: addr.splits cell.splits simp: mext nth_list_update')
+    by (auto split: addr.splits block.splits simp: mext nth_list_update')
   
-    
-  definition "addr_alloc vs b m \<equiv> mmap m b (\<lambda>_. BLOCK vs)"  
+  subsection \<open>Allocating and Freeing\<close>  
+  definition "addr_alloc vs b m \<equiv> mmap m b (\<lambda>_. ALLOC vs)"  
   definition "addr_free b m \<equiv> mmap m b (\<lambda>_. FREED)"  
 
   lemma addr_alloc_state[simp]:
@@ -154,7 +189,7 @@ begin
     "is_FRESH (put_addr m a x) b' \<longleftrightarrow> is_FRESH m b'"  
     "is_ALLOC (put_addr m a x) b' \<longleftrightarrow> is_ALLOC m b'"  
     "is_FREED (put_addr m a x) b' \<longleftrightarrow> is_FREED m b'"
-    by (auto simp: put_addr_def split: addr.splits cell.splits)
+    by (auto simp: put_addr_def split: addr.splits block.splits)
     
     
   
@@ -182,51 +217,33 @@ begin
     "is_valid_ptr_addr (addr_free b m) a = (addr.block a \<noteq> b \<and> is_valid_ptr_addr m a)"
     by (cases a; auto simp: is_valid_addr_def is_valid_ptr_addr_def)+
     
-  definition list_combine where
-    "list_combine xs\<^sub>1 I xs\<^sub>2 \<equiv> map (\<lambda>i. if i\<in>I then xs\<^sub>2!i else xs\<^sub>1!i) [0..<length xs\<^sub>1 ]"
+  subsection \<open>Combining Memories\<close>  
+  text \<open>The definition of the raw combine operator is asymmetric,
+    using the first memory by default, except for some specified blocks and addresses.
+    Symmetry is only proved later, when we know that the combined memories have actually evolved by
+    consistent, race-free executions.
+  \<close>
     
-  lemma nth_undefined: "\<not>i<length xs \<Longrightarrow> xs!i = undefined (i-length xs)"
-    apply (induction xs arbitrary: i)
-    apply (simp add: nth_def)
-    by auto
+  fun block_combine where
+    "block_combine FRESH I c = c"
+  | "block_combine c I FRESH = c"
+  | "block_combine FREED I c = FREED"
+  | "block_combine c I FREED = FREED"
+  | "block_combine (ALLOC vs\<^sub>1) I (ALLOC vs\<^sub>2) = ALLOC (list_combine vs\<^sub>1 I vs\<^sub>2)"
     
-  lemma list_combine_nth: "length xs\<^sub>1 = length xs\<^sub>2 \<Longrightarrow> list_combine xs\<^sub>1 I xs\<^sub>2 ! i = (if i\<in>I then xs\<^sub>2!i else xs\<^sub>1!i)"  
-    unfolding list_combine_def
-    apply (cases "i<length xs\<^sub>2")
-    subgoal by (auto simp: )
-    subgoal by (simp add: nth_undefined)
-    done
-
-  lemma list_combine_length[simp]: "length (list_combine xs\<^sub>1 I xs\<^sub>2) = length xs\<^sub>1"  
-    by (auto simp: list_combine_def)
-    
-  lemma list_combine_inth: "length xs\<^sub>1 = length xs\<^sub>2 \<Longrightarrow> i_nth (list_combine xs\<^sub>1 I xs\<^sub>2) i = (if nat i\<in>I then i_nth xs\<^sub>2 i else i_nth xs\<^sub>1 i)"  
-    apply (cases "0\<le>i"; simp)
-    apply (cases "nat i < length xs\<^sub>1"; auto simp: list_combine_nth)
-    done
-    
-    
-    
-  fun cell_combine where
-    "cell_combine FRESH I c = c"
-  | "cell_combine c I FRESH = c"
-  | "cell_combine FREED I c = FREED"
-  | "cell_combine c I FREED = FREED"
-  | "cell_combine (BLOCK vs\<^sub>1) I (BLOCK vs\<^sub>2) = BLOCK (list_combine vs\<^sub>1 I vs\<^sub>2)"
-    
-  lemma cell_combine_add_simps[simp]:
-    "cell_combine c I FRESH = c"
-    "cell_combine FREED I c = FREED"
-    "cell_combine c I FREED = FREED"
+  lemma block_combine_add_simps[simp]:
+    "block_combine c I FRESH = c"
+    "block_combine FREED I c = FREED"
+    "block_combine c I FREED = FREED"
     by (cases c; simp)+
   
   lift_definition mcombine :: "('v) memory \<Rightarrow> (addr set) \<Rightarrow> ('v) memory \<Rightarrow> ('v) memory" is
-    "\<lambda>m\<^sub>1 A m\<^sub>2 b. cell_combine (m\<^sub>1 b) { nat i | i. 0\<le>i \<and> ADDR b i \<in> A} (m\<^sub>2 b)"
+    "\<lambda>m\<^sub>1 A m\<^sub>2 b. block_combine (m\<^sub>1 b) { nat i | i. 0\<le>i \<and> ADDR b i \<in> A} (m\<^sub>2 b)"
     subgoal for f\<^sub>1 A f\<^sub>2
     proof goal_cases
       case 1
       
-      have "{b. cell_combine (f\<^sub>1 b) {nat i | i. 0\<le>i \<and> ADDR b i \<in> A} (f\<^sub>2 b) \<noteq> FRESH} \<subseteq> {a. f\<^sub>1 a \<noteq> FRESH} \<union> {a. f\<^sub>2 a \<noteq> FRESH}"
+      have "{b. block_combine (f\<^sub>1 b) {nat i | i. 0\<le>i \<and> ADDR b i \<in> A} (f\<^sub>2 b) \<noteq> FRESH} \<subseteq> {a. f\<^sub>1 a \<noteq> FRESH} \<union> {a. f\<^sub>2 a \<noteq> FRESH}"
         by auto
         
       from finite_subset[OF this] 1 show ?case by auto
@@ -234,7 +251,7 @@ begin
   done
     
   
-  lemma mapp_combine[simp]: "mapp (mcombine m\<^sub>1 A m\<^sub>2) b = cell_combine (mapp m\<^sub>1 b) { nat i | i. 0\<le>i \<and> ADDR b i \<in> A} (mapp m\<^sub>2 b)"
+  lemma mapp_combine[simp]: "mapp (mcombine m\<^sub>1 A m\<^sub>2) b = block_combine (mapp m\<^sub>1 b) { nat i | i. 0\<le>i \<and> ADDR b i \<in> A} (mapp m\<^sub>2 b)"
     apply transfer
     by auto  
 
@@ -247,58 +264,60 @@ begin
     by (metis (mono_tags, lifting) finite_compl infinite_UNIV rev_finite_subset subset_Collect_conv)
       
 
-  (* Valid transitions of memory cells *)  
-  definition "cell_state_trans c c' \<equiv> 
-    (cell.is_block c \<longrightarrow> (cell.is_block c' \<and> length (cell.vals c') = length (cell.vals c)) \<or> c'=FREED)
+  subsection \<open>Valid State Transitions of Memory Blocks\<close>  
+  text \<open>Blocks can only transition from fresh to allocated to freed, and 
+    allocated blocks cannot change their size.
+  \<close>
+  
+  definition "block_state_trans c c' \<equiv> 
+    (block.is_alloc c \<longrightarrow> (block.is_alloc c' \<and> length (block.vals c') = length (block.vals c)) \<or> c'=FREED)
   \<and> (c=FREED \<longrightarrow> c'=FREED)"
 
       
   (* Alternative characterization: *)  
-  inductive cell_state_trans1 where
-    "cell_state_trans1 FRESH (BLOCK vs)" 
-  | "length vs' = length vs \<Longrightarrow> cell_state_trans1 (BLOCK vs) (BLOCK vs')" 
-  | "cell_state_trans1 (BLOCK vs) FREED"
+  inductive block_state_trans1 where
+    "block_state_trans1 FRESH (ALLOC vs)" 
+  | "length vs' = length vs \<Longrightarrow> block_state_trans1 (ALLOC vs) (ALLOC vs')" 
+  | "block_state_trans1 (ALLOC vs) FREED"
     
   (* TODO: Move *)  
   lemma r2_into_rtranclp: "P a b \<Longrightarrow> P b c \<Longrightarrow> P\<^sup>*\<^sup>* a c" by auto
     
-  lemma cell_state_trans_alt: "cell_state_trans c c' = cell_state_trans1\<^sup>*\<^sup>* c c'"
+  lemma block_state_trans_alt: "block_state_trans c c' = block_state_trans1\<^sup>*\<^sup>* c c'"
   proof
-    show "cell_state_trans1\<^sup>*\<^sup>* c c' \<Longrightarrow> cell_state_trans c c'"
+    show "block_state_trans1\<^sup>*\<^sup>* c c' \<Longrightarrow> block_state_trans c c'"
       apply (induction rule: rtranclp.induct)
-      unfolding cell_state_trans_def
-      by (auto elim: cell_state_trans1.cases)
+      unfolding block_state_trans_def
+      by (auto elim: block_state_trans1.cases)
   
-    show "cell_state_trans c c' \<Longrightarrow> cell_state_trans1\<^sup>*\<^sup>* c c'"  
-      unfolding cell_state_trans_def
+    show "block_state_trans c c' \<Longrightarrow> block_state_trans1\<^sup>*\<^sup>* c c'"  
+      unfolding block_state_trans_def
       apply (cases c; cases c'; simp)
-      apply (auto intro: r2_into_rtranclp cell_state_trans1.intros)
+      apply (auto intro: r2_into_rtranclp block_state_trans1.intros)
       done
     
   qed    
   
-
-  
-  lemma cell_state_trans_simps[simp]:
-    "cell_state_trans c c"
-    "cell_state_trans FRESH c"
-    "cell_state_trans c FREED"
-    "cell_state_trans (BLOCK vs) (BLOCK vs') \<longleftrightarrow> length vs' = length vs"
-    "cell_state_trans FREED c' \<longleftrightarrow> c'=FREED"
-    by (auto simp: cell_state_trans_def)
+  lemma block_state_trans_simps[simp]:
+    "block_state_trans c c"
+    "block_state_trans FRESH c"
+    "block_state_trans c FREED"
+    "block_state_trans (ALLOC vs) (ALLOC vs') \<longleftrightarrow> length vs' = length vs"
+    "block_state_trans FREED c' \<longleftrightarrow> c'=FREED"
+    by (auto simp: block_state_trans_def)
   
       
-  lemma cell_state_trans_trans[trans]: "cell_state_trans c c' \<Longrightarrow> cell_state_trans c' c'' \<Longrightarrow> cell_state_trans c c''"  
-    by (auto simp: cell_state_trans_def)
+  lemma block_state_trans_trans[trans]: "block_state_trans c c' \<Longrightarrow> block_state_trans c' c'' \<Longrightarrow> block_state_trans c c''"  
+    by (auto simp: block_state_trans_def)
   
   
   definition "valid_block_trans m m' b \<equiv> 
       (is_ALLOC m b \<longrightarrow> (is_ALLOC m' b \<and> block_size m' b = block_size m b) \<or> is_FREED m' b)
     \<and> (is_FREED m b \<longrightarrow> is_FREED m' b)"  
     
-  lemma valid_block_trans_alt: "valid_block_trans m m' b \<longleftrightarrow> cell_state_trans (mapp m b) (mapp m' b)"  
-    unfolding valid_block_trans_def cell_state_trans_def block_size_def
-    by (auto split: cell.split)
+  lemma valid_block_trans_alt: "valid_block_trans m m' b \<longleftrightarrow> block_state_trans (mapp m b) (mapp m' b)"  
+    unfolding valid_block_trans_def block_state_trans_def block_size_def
+    by (auto split: block.split)
     
 
   lemma valid_block_trans_refl[simp]:
@@ -334,62 +353,64 @@ begin
   lemma freed_blocks_refl[simp]: "freed_blocks m m = {}"
     by (auto simp: freed_blocks_def)
       
-  
-  datatype intf = interference 
+
+  subsection \<open>Access Reports\<close>
+      
+  datatype acc = ACC_REPORT 
     (r: "addr set")   \<comment> \<open>Read addresses\<close>
     (w: "addr set")   \<comment> \<open>Written addresses\<close>
-    (a: "block set")  \<comment> \<open>Allocated blocks\<close>
-    (f: "block set")  \<comment> \<open>Freed blocks\<close>
+    (a: "block_idx set")  \<comment> \<open>Allocated blocks\<close>
+    (f: "block_idx set")  \<comment> \<open>Freed blocks\<close>
     
   hide_const (open) r w a f
     
-  text \<open>These ensure that e contains all referenced blocks\<close>
-  abbreviation "intf_r r \<equiv> interference {r} {} {} {}" 
-  abbreviation "intf_w w \<equiv> interference {} {w} {} {}" 
-  abbreviation "intf_a a \<equiv> interference {} {}  {a} {}" 
-  abbreviation "intf_f f \<equiv> interference {} {}  {} {f}" 
+  abbreviation "acc_r r \<equiv> ACC_REPORT {r} {} {} {}" 
+  abbreviation "acc_w w \<equiv> ACC_REPORT {} {w} {} {}" 
+  abbreviation "acc_a a \<equiv> ACC_REPORT {} {}  {a} {}" 
+  abbreviation "acc_f f \<equiv> ACC_REPORT {} {}  {} {f}" 
   
   
-  instantiation intf :: comm_monoid_add
+  instantiation acc :: comm_monoid_add
   begin
-    definition "0 = interference {} {} {} {}"
-    definition "a+b \<equiv> case (a,b) of (interference ra wa aa fa, interference rb wb ab fb) \<Rightarrow>
-      interference (ra\<union>rb) (wa\<union>wb) (aa\<union>ab) (fa\<union>fb)"
+    definition "0 = ACC_REPORT {} {} {} {}"
+    definition "a+b \<equiv> case (a,b) of (ACC_REPORT ra wa aa fa, ACC_REPORT rb wb ab fb) \<Rightarrow>
+      ACC_REPORT (ra\<union>rb) (wa\<union>wb) (aa\<union>ab) (fa\<union>fb)"
 
      instance
        apply standard     
-       unfolding zero_intf_def plus_intf_def
-       by (auto split: intf.split)
+       unfolding zero_acc_def plus_acc_def
+       by (auto split: acc.split)
       
   end
   
     
-  lemma intf_zero_simps[simp]:  
-    "intf.r 0 = {}"  
-    "intf.w 0 = {}"  
-    "intf.a 0 = {}"  
-    "intf.f 0 = {}"  
-    by (auto split: intf.split simp: zero_intf_def)
+  lemma acc_zero_simps[simp]:  
+    "acc.r 0 = {}"  
+    "acc.w 0 = {}"  
+    "acc.a 0 = {}"  
+    "acc.f 0 = {}"  
+    by (auto split: acc.split simp: zero_acc_def)
     
-  lemma intf_plus_simps[simp]:
-    "intf.r (a+b) = intf.r a \<union> intf.r b"  
-    "intf.w (a+b) = intf.w a \<union> intf.w b"  
-    "intf.a (a+b) = intf.a a \<union> intf.a b"  
-    "intf.f (a+b) = intf.f a \<union> intf.f b"  
-    by (auto split: intf.split simp: plus_intf_def)
+  lemma acc_plus_simps[simp]:
+    "acc.r (a+b) = acc.r a \<union> acc.r b"  
+    "acc.w (a+b) = acc.w a \<union> acc.w b"  
+    "acc.a (a+b) = acc.a a \<union> acc.a b"  
+    "acc.f (a+b) = acc.f a \<union> acc.f b"  
+    by (auto split: acc.split simp: plus_acc_def)
   
-  abbreviation "split_intf i \<equiv> (
-    intf.r i, 
-    intf.w i, 
-    intf.a i, 
-    intf.f i
+  abbreviation "split_acc i \<equiv> (
+    acc.r i, 
+    acc.w i, 
+    acc.a i, 
+    acc.f i
   )"
   
 
-  text \<open>Reported interference is consistent with observable state change. 
+  subsubsection \<open>Consistency with Memory Change\<close>
+  text \<open>Reported ACC_REPORT is consistent with observable state change. 
     Also includes that state change itself is consistent.\<close>
-  definition "intf_consistent s i s' \<equiv> 
-    let (r,w,a,f) = split_intf i in
+  definition "acc_consistent s i s' \<equiv> 
+    let (r,w,a,f) = split_acc i in
       \<comment> \<open>Referred to blocks must exist or have existed in final state, and cannot be freed in initial state\<close>
       (\<forall>b \<in> addr.block`(r\<union>w) \<union> a \<union> f. \<not>is_FRESH s' b \<and> \<not>is_FREED s b) 
       \<comment> \<open>Read and written addresses must be valid\<close>
@@ -405,44 +426,16 @@ begin
     \<and> (\<forall>a. is_valid_addr s a \<and> is_valid_addr s' a \<and> a\<notin>w \<longrightarrow> get_addr s a = get_addr s' a)
   "
 
-  text \<open>Parallel state changes are feasible: the memory manager did not allocate the same blocks\<close>    
-  definition "spar_feasible i\<^sub>1 i\<^sub>2 \<equiv> intf.a i\<^sub>1 \<inter> intf.a i\<^sub>2 = {}"
-  
-  text \<open>Parallel executions have no race.
-    Note, that this assumes that the interference report is consistent
-  \<close>      
-  definition "intf_norace i\<^sub>1 i\<^sub>2 \<equiv> 
-    let (r\<^sub>1, w\<^sub>1, a\<^sub>1, f\<^sub>1) = split_intf i\<^sub>1 in
-    let (r\<^sub>2, w\<^sub>2, a\<^sub>2, f\<^sub>2) = split_intf i\<^sub>2 in
-    let m\<^sub>1 = w\<^sub>1 \<union> {a. addr.block a \<in> f\<^sub>1} in
-    let m\<^sub>2 = w\<^sub>2 \<union> {a. addr.block a \<in> f\<^sub>2} in
-      \<comment> \<open>Addresses read or modified by thread1 not modified by thread2\<close>
-      (r\<^sub>1\<union>m\<^sub>1) \<inter> (m\<^sub>2) = {}
-      \<comment> \<open>Addresses modified by thread1 not read or modified by thread2\<close>
-    \<and> (m\<^sub>1) \<inter> (r\<^sub>2\<union>m\<^sub>2) = {}
-    "
-  
-  (* TODO: Stronger version of no-race as lemma, 
-    assuming intf_consistent + feasible!
-  *)  
-    
-  definition "combine_states s\<^sub>1 i\<^sub>2 s\<^sub>2 \<equiv> mcombine s\<^sub>1 (intf.w i\<^sub>2) s\<^sub>2"
-
-  lemma spar_feasible_sym: "spar_feasible i\<^sub>1 i\<^sub>2 = spar_feasible i\<^sub>2 i\<^sub>1"  
-    by (auto simp: spar_feasible_def)
-
-  lemma intf_norace_sym: "intf_norace i\<^sub>1 i\<^sub>2 = intf_norace i\<^sub>2 i\<^sub>1"  
-    by (simp add: intf_norace_def Let_def; fast)
-    
-  locale intf_consistent_loc =
+  text \<open>For convenience, we define locales for consistent executions\<close>
+  locale acc_consistent_loc =
     fixes s i s'
-    assumes consistent: "intf_consistent s i s'"
+    assumes consistent: "acc_consistent s i s'"
   begin
-    abbreviation "r \<equiv> intf.r i"
-    abbreviation "w \<equiv> intf.w i"
-    abbreviation "a \<equiv> intf.a i"
-    abbreviation "f \<equiv> intf.f i"
-    abbreviation "m \<equiv> intf.w i \<union> {addr. addr.block addr \<in> f}"
+    abbreviation "r \<equiv> acc.r i"
+    abbreviation "w \<equiv> acc.w i"
+    abbreviation "a \<equiv> acc.a i"
+    abbreviation "f \<equiv> acc.f i"
+    abbreviation "m \<equiv> acc.w i \<union> {addr. addr.block addr \<in> f}"
 
     
     abbreviation "allocated_addrs_approx \<equiv> {addr. addr.block addr \<in> a}"
@@ -451,48 +444,48 @@ begin
     
     lemma valid_block_trans: 
       "valid_block_trans s s' b"
-      using consistent unfolding intf_consistent_def by auto
+      using consistent unfolding acc_consistent_def by auto
   
-    lemma intf_a_alloc: 
+    lemma acc_a_alloc: 
       "a = alloc_blocks s s'"  
-      using consistent unfolding intf_consistent_def by auto
+      using consistent unfolding acc_consistent_def by auto
       
-    lemma intf_f_freed: 
+    lemma acc_f_freed: 
       "f = freed_blocks s s'"  
-      using consistent unfolding intf_consistent_def by auto
+      using consistent unfolding acc_consistent_def by auto
       
-    lemma intf_ref_not_fresh:  
+    lemma acc_ref_not_fresh:  
       "b\<in>addr.block ` (r \<union> w) \<union> a \<union> f \<Longrightarrow> mapp s' b \<noteq> FRESH"
-      using consistent unfolding intf_consistent_def by auto
+      using consistent unfolding acc_consistent_def by auto
 
-    lemma intf_ref_not_freed:  
+    lemma acc_ref_not_freed:  
       "b\<in>addr.block ` (r \<union> w) \<union> a \<union> f \<Longrightarrow> mapp s b \<noteq> FREED"
-      using consistent unfolding intf_consistent_def by auto
+      using consistent unfolding acc_consistent_def by auto
           
-    lemma intf_nw_untouched:  
+    lemma acc_nw_untouched:  
       "is_valid_addr s addr \<Longrightarrow> is_valid_addr s' addr \<Longrightarrow> addr \<notin> w \<Longrightarrow> get_addr s' addr = get_addr s addr"
-      using consistent unfolding intf_consistent_def by auto
+      using consistent unfolding acc_consistent_def by auto
 
     lemma valid_if_not_freed: "is_valid_addr s addr \<Longrightarrow> addr.block addr \<notin> f \<Longrightarrow> is_valid_addr s' addr"
       apply (cases addr; clarsimp)
       subgoal for b i
         using valid_block_trans[of b]
         unfolding is_valid_addr_def valid_block_trans_def
-        by (auto simp: intf_f_freed freed_blocks_def)
+        by (auto simp: acc_f_freed freed_blocks_def)
       done
 
     lemma rw_valid_s:  
       "addr\<in>r\<union>w \<Longrightarrow> is_ALLOC s (addr.block addr) \<Longrightarrow> is_valid_addr s addr"
-      using consistent unfolding intf_consistent_def by auto
+      using consistent unfolding acc_consistent_def by auto
     
     lemma rw_valid_s':  
       "addr\<in>r\<union>w \<Longrightarrow> is_ALLOC s' (addr.block addr) \<Longrightarrow> is_valid_addr s' addr"
-      using consistent unfolding intf_consistent_def by auto
+      using consistent unfolding acc_consistent_def by auto
     
             
     lemma addr_orig_val: "is_valid_addr s addr \<Longrightarrow> addr.block addr \<notin> f \<Longrightarrow> addr\<notin>w 
       \<Longrightarrow> is_valid_addr s' addr \<and> get_addr s' addr = get_addr s addr"
-      using intf_nw_untouched valid_if_not_freed by blast
+      using acc_nw_untouched valid_if_not_freed by blast
       
     lemma valid_trans_imps:
       "is_FREED s b \<Longrightarrow> is_FREED s' b"  
@@ -500,21 +493,21 @@ begin
       "is_FRESH s' b \<Longrightarrow> is_FRESH s b"  
       using valid_block_trans[of b]
       apply (auto simp: valid_block_trans_def)
-      using cell.exhaust_disc by blast
+      using block.exhaust_disc by blast
       
 
     lemma is_ALLOC'_eq: "is_ALLOC s' b \<longleftrightarrow> b\<notin>f \<and> (is_ALLOC s b \<or> b \<in> a)"  
-      unfolding intf_a_alloc intf_f_freed alloc_blocks_def freed_blocks_def
+      unfolding acc_a_alloc acc_f_freed alloc_blocks_def freed_blocks_def
       apply simp
-      by (metis cell.disc(2) cell.exhaust_disc valid_trans_imps(1) valid_trans_imps(2))
+      by (metis block.disc(2) block.exhaust_disc valid_trans_imps(1) valid_trans_imps(2))
       
     lemma is_FRESH'_eq: "is_FRESH s' b \<longleftrightarrow> b\<notin>a \<and> is_FRESH s b"  
-      unfolding intf_a_alloc intf_f_freed alloc_blocks_def freed_blocks_def
+      unfolding acc_a_alloc acc_f_freed alloc_blocks_def freed_blocks_def
       apply simp
       using valid_trans_imps(3) by blast
       
     lemma is_FREED'_eq: "is_FREED s' b \<longleftrightarrow> is_FREED s b \<or> b\<in>f"  
-      unfolding intf_a_alloc intf_f_freed alloc_blocks_def freed_blocks_def
+      unfolding acc_a_alloc acc_f_freed alloc_blocks_def freed_blocks_def
       apply simp
       using valid_trans_imps(1) by blast
       
@@ -527,7 +520,7 @@ begin
       
       assume A: "addr \<in> r \<union> w"
       
-      with intf_ref_not_freed[of b] intf_ref_not_fresh[of b] 
+      with acc_ref_not_freed[of b] acc_ref_not_fresh[of b] 
       have "\<not>is_FREED s b" "\<not>is_FRESH s' b" by force+
       hence "b\<in>a \<or> is_ALLOC s b" 
         by (auto simp: is_FRESH'_eq is_ALLOC_conv)
@@ -536,10 +529,10 @@ begin
     qed done
 
     lemma f_valid_or_alloc: "f \<subseteq> Collect (is_ALLOC s) \<union> a"
-      by (smt (verit, del_insts) Collect_mono_iff UnI2 freed_blocks_def intf_f_freed is_ALLOC_conv is_FRESH'_eq mem_Collect_eq sup_ge1 sup_set_def)
+      by (smt (verit, del_insts) Collect_mono_iff UnI2 freed_blocks_def acc_f_freed is_ALLOC_conv is_FRESH'_eq mem_Collect_eq sup_ge1 sup_set_def)
     
     lemma a_dj_alloc: "Collect (is_ALLOC s) \<inter> a = {}"  
-      unfolding intf_a_alloc alloc_blocks_def
+      unfolding acc_a_alloc alloc_blocks_def
       by (auto)
           
     lemma a_dj_valid: "Collect (is_valid_addr s) \<inter> {addr. addr.block addr \<in> a} = {}"  
@@ -547,8 +540,8 @@ begin
       by (auto split: addr.splits)
       
     lemma valid_addrs'_subset: "Collect (is_valid_addr s') \<subseteq> Collect (is_valid_addr s) \<union> allocated_addrs_approx"
-      apply (auto simp: intf_a_alloc)
-      by (smt addr.case_eq_if cell.disc(2) intf_a_alloc is_ALLOC'_eq 
+      apply (auto simp: acc_a_alloc)
+      by (smt addr.case_eq_if block.disc(2) acc_a_alloc is_ALLOC'_eq 
               valid_block_trans  is_valid_addr_alt valid_block_trans_def)
       
     definition "allocated_addrs \<equiv> Collect (is_valid_addr s') - Collect (is_valid_addr s)"      
@@ -589,57 +582,97 @@ begin
       
             
   end  
-    
-  lemma intf_consistent_trans:  
-    assumes "intf_consistent s i\<^sub>1 s\<^sub>1" 
-    assumes "intf_consistent s\<^sub>1 i\<^sub>2 s\<^sub>2"  
-    shows "intf_consistent s (i\<^sub>1 + i\<^sub>2) s\<^sub>2"
+
+  text \<open>Consistency is transitive\<close>    
+  lemma acc_consistent_trans:  
+    assumes "acc_consistent s i\<^sub>1 s\<^sub>1" 
+    assumes "acc_consistent s\<^sub>1 i\<^sub>2 s\<^sub>2"  
+    shows "acc_consistent s (i\<^sub>1 + i\<^sub>2) s\<^sub>2"
   proof -
-    interpret c1: intf_consistent_loc s i\<^sub>1 s\<^sub>1 by unfold_locales fact
-    interpret c2: intf_consistent_loc s\<^sub>1 i\<^sub>2 s\<^sub>2 by unfold_locales fact
+    interpret c1: acc_consistent_loc s i\<^sub>1 s\<^sub>1 by unfold_locales fact
+    interpret c2: acc_consistent_loc s\<^sub>1 i\<^sub>2 s\<^sub>2 by unfold_locales fact
   
     show ?thesis
-      unfolding intf_consistent_def Let_def split
+      unfolding acc_consistent_def Let_def split
       apply (intro conjI allI ballI)
       subgoal for b
-        using c1.intf_ref_not_fresh[of b] c2.intf_ref_not_fresh[of b]
+        using c1.acc_ref_not_fresh[of b] c2.acc_ref_not_fresh[of b]
         by (auto simp: c1.is_FRESH'_eq c2.is_FRESH'_eq)
       subgoal for b
-        using c1.intf_ref_not_freed[of b] c2.intf_ref_not_freed[of b]
+        using c1.acc_ref_not_freed[of b] c2.acc_ref_not_freed[of b]
         by (auto simp: c1.is_FREED'_eq)
       subgoal for a
         using c1.rw_valid_s[of a] c1.rw_valid_s'[of a] c2.rw_valid_s[of a]
         apply clarsimp
-        apply (smt (verit, ccfv_threshold) Un_iff addr.case_eq_if c1.valid_block_trans c2.intf_ref_not_freed image_eqI is_valid_addr_def valid_block_trans_def)
+        apply (smt (verit, ccfv_threshold) Un_iff addr.case_eq_if c1.valid_block_trans c2.acc_ref_not_freed image_eqI is_valid_addr_def valid_block_trans_def)
         done
       subgoal for a
         using c1.rw_valid_s'[of a] c2.rw_valid_s'[of a] c2.rw_valid_s[of a]
         apply clarsimp
-        by (metis Un_iff c1.intf_ref_not_fresh c2.is_ALLOC'_eq c2.is_FREED'_eq c2.valid_if_not_freed cell.exhaust_disc image_subset_iff sup_ge1)
+        by (metis Un_iff c1.acc_ref_not_fresh c2.is_ALLOC'_eq c2.is_FREED'_eq c2.valid_if_not_freed block.exhaust_disc image_subset_iff sup_ge1)
       subgoal
         using c1.valid_block_trans c2.valid_block_trans valid_block_trans_trans by blast
       subgoal
-        apply (simp add: c1.intf_a_alloc c2.intf_a_alloc alloc_blocks_def)
+        apply (simp add: c1.acc_a_alloc c2.acc_a_alloc alloc_blocks_def)
         by (auto simp: c1.is_FRESH'_eq c2.is_FRESH'_eq)
       subgoal
-        apply (simp add: c1.intf_f_freed c2.intf_f_freed freed_blocks_def)
+        apply (simp add: c1.acc_f_freed c2.acc_f_freed freed_blocks_def)
         by (auto simp: c1.is_FREED'_eq c2.is_FREED'_eq)
       subgoal
-        by (smt (verit, del_insts) Un_iff addr.case_eq_if block_size_noblock(2) c1.intf_nw_untouched c1.is_FREED'_eq c1.valid_if_not_freed c2.intf_nw_untouched c2.is_FREED'_eq intf_plus_simps(2) is_valid_addr_def)
+        by (smt (verit, del_insts) Un_iff addr.case_eq_if block_size_noblock(2) c1.acc_nw_untouched c1.is_FREED'_eq c1.valid_if_not_freed c2.acc_nw_untouched c2.is_FREED'_eq acc_plus_simps(2) is_valid_addr_def)
       done
   qed  
 
+  
+  
+  
+  subsection \<open>Parallel Execution\<close>
+  
+  subsubsection \<open>Feasibility and Data Race\<close>
+  
+  text \<open>Parallel state changes are feasible: the memory manager did not allocate the same blocks\<close>    
+  definition "spar_feasible i\<^sub>1 i\<^sub>2 \<equiv> acc.a i\<^sub>1 \<inter> acc.a i\<^sub>2 = {}"
+  
+  text \<open>Parallel executions have no race.
+    Note, that this assumes that the ACC_REPORT report is consistent.
+    See lemma \<open>acc_norace_strong\<close> below for alternative definition 
+    including allocated blocks.
+  \<close>      
+  definition "acc_norace i\<^sub>1 i\<^sub>2 \<equiv> 
+    let (r\<^sub>1, w\<^sub>1, a\<^sub>1, f\<^sub>1) = split_acc i\<^sub>1 in
+    let (r\<^sub>2, w\<^sub>2, a\<^sub>2, f\<^sub>2) = split_acc i\<^sub>2 in
+    let m\<^sub>1 = w\<^sub>1 \<union> {a. addr.block a \<in> f\<^sub>1} in
+    let m\<^sub>2 = w\<^sub>2 \<union> {a. addr.block a \<in> f\<^sub>2} in
+      \<comment> \<open>Addresses read or modified by thread1 not modified by thread2\<close>
+      (r\<^sub>1\<union>m\<^sub>1) \<inter> (m\<^sub>2) = {}
+      \<comment> \<open>Addresses modified by thread1 not read or modified by thread2\<close>
+    \<and> (m\<^sub>1) \<inter> (r\<^sub>2\<union>m\<^sub>2) = {}
+    "
+  
+  
+  
+  lemma spar_feasible_sym: "spar_feasible i\<^sub>1 i\<^sub>2 = spar_feasible i\<^sub>2 i\<^sub>1"  
+    by (auto simp: spar_feasible_def)
+
+  lemma acc_norace_sym: "acc_norace i\<^sub>1 i\<^sub>2 = acc_norace i\<^sub>2 i\<^sub>1"  
+    by (simp add: acc_norace_def Let_def; fast)
+    
+  
+  definition "combine_states s\<^sub>1 i\<^sub>2 s\<^sub>2 \<equiv> mcombine s\<^sub>1 (acc.w i\<^sub>2) s\<^sub>2"
+
+  
+  text \<open>Locale that assumes consistent, feasible parallel executions\<close>
   locale feasible_parallel_execution =
     fixes s s\<^sub>1 i\<^sub>1 s\<^sub>2 i\<^sub>2
-    assumes c1[simp]: "intf_consistent s i\<^sub>1 s\<^sub>1"
-    assumes c2[simp]: "intf_consistent s i\<^sub>2 s\<^sub>2"
+    assumes c1[simp]: "acc_consistent s i\<^sub>1 s\<^sub>1"
+    assumes c2[simp]: "acc_consistent s i\<^sub>2 s\<^sub>2"
     assumes feasible: "spar_feasible i\<^sub>1 i\<^sub>2"
   begin  
   
-    sublocale c1: intf_consistent_loc s i\<^sub>1 s\<^sub>1
+    sublocale c1: acc_consistent_loc s i\<^sub>1 s\<^sub>1
       by unfold_locales (rule c1)
     
-    sublocale c2: intf_consistent_loc s i\<^sub>2 s\<^sub>2
+    sublocale c2: acc_consistent_loc s i\<^sub>2 s\<^sub>2
       by unfold_locales (rule c2)
 
   
@@ -666,14 +699,14 @@ begin
       have "b \<in> alloc_blocks s s\<^sub>1 \<inter> alloc_blocks s s\<^sub>2"
         unfolding alloc_blocks_def by auto
       with feasible have False
-        unfolding spar_feasible_def c1.intf_a_alloc c2.intf_a_alloc by auto
+        unfolding spar_feasible_def c1.acc_a_alloc c2.acc_a_alloc by auto
       then show ?thesis ..
     next
       case FREED
       with c1.valid_block_trans[of b] have False unfolding valid_block_trans_def by auto
       then show ?thesis ..
     next
-      case (BLOCK vs)
+      case (ALLOC vs)
       then show ?thesis by simp
     qed
     
@@ -681,7 +714,7 @@ begin
       assumes "is_ALLOC s\<^sub>1 b" 
       assumes "is_ALLOC s\<^sub>2 b"  
       shows "block_size s\<^sub>1 b = block_size s\<^sub>2 b"  
-      by (metis assms(1) assms(2) c1.valid_block_trans c2.valid_block_trans cell.disc(2) par_blocks_exist_before valid_block_trans_def)
+      by (metis assms(1) assms(2) c1.valid_block_trans c2.valid_block_trans block.disc(2) par_blocks_exist_before valid_block_trans_def)
         
     lemma block_size_combine[simp]: "block_size (mcombine s\<^sub>1 A s\<^sub>2) b = (
       if is_ALLOC s\<^sub>1 b \<and> \<not>is_FREED s\<^sub>2 b then block_size s\<^sub>1 b
@@ -707,7 +740,7 @@ begin
     abbreviation "s' \<equiv> combine_states s\<^sub>1 i\<^sub>2 s\<^sub>2"                                              
 
     (* TODO: Move *)
-    lemma cell_combine_FRESH_iff[simp]: "cell_combine c\<^sub>1 A c\<^sub>2 = FRESH \<longleftrightarrow> c\<^sub>1=FRESH \<and> c\<^sub>2=FRESH"
+    lemma block_combine_FRESH_iff[simp]: "block_combine c\<^sub>1 A c\<^sub>2 = FRESH \<longleftrightarrow> c\<^sub>1=FRESH \<and> c\<^sub>2=FRESH"
       by (cases c\<^sub>1; cases c\<^sub>2; simp)
 
     lemma is_FRESH'_eq: "is_FRESH s' b \<longleftrightarrow> is_FRESH s\<^sub>1 b \<and> is_FRESH s\<^sub>2 b \<and> b\<notin>a\<^sub>1\<union>a\<^sub>2"  
@@ -715,21 +748,21 @@ begin
       
     lemma is_ALLOC'_eq: "is_ALLOC s' b \<longleftrightarrow> (b\<notin>f\<^sub>1\<union>f\<^sub>2) \<and> (b\<in>a\<^sub>1\<union>a\<^sub>2 \<or> is_ALLOC s b)"  
       apply (auto simp: combine_states_def)
-      subgoal by (smt (verit, best) c1.is_FREED'_eq cell.disc(2) cell_combine_add_simps(2))
-      subgoal by (metis (no_types, lifting) c2.is_FREED'_eq cell.disc(2) cell_combine_add_simps(3))
-      subgoal by (smt (z3) c1.is_ALLOC'_eq c2.is_ALLOC'_eq cell_combine.simps(1) cell_combine_add_simps(2) is_ALLOC_conv)
+      subgoal by (smt (verit, best) c1.is_FREED'_eq block.disc(2) block_combine_add_simps(2))
+      subgoal by (metis (no_types, lifting) c2.is_FREED'_eq block.disc(2) block_combine_add_simps(3))
+      subgoal by (smt (z3) c1.is_ALLOC'_eq c2.is_ALLOC'_eq block_combine.simps(1) block_combine_add_simps(2) is_ALLOC_conv)
 
-      subgoal by (metis (mono_tags, lifting) alloc_blocks_def c1.intf_a_alloc c1.is_ALLOC'_eq c2.is_FREED'_eq cell.distinct_disc(4) cell.exhaust_disc cell_combine_add_simps(1) mem_Collect_eq par_blocks_exist_before)
-      subgoal by (smt (z3) c1.is_FREED'_eq c2.is_ALLOC'_eq c2.is_FREED'_eq cell.exhaust_disc cell_combine.simps(1) cell_combine.simps(7) is_block_def) 
-      subgoal by (metis (no_types, lifting) c1.is_ALLOC'_eq c2.is_ALLOC'_eq cell_combine.simps(7) is_block_def)
+      subgoal by (metis (mono_tags, lifting) alloc_blocks_def c1.acc_a_alloc c1.is_ALLOC'_eq c2.is_FREED'_eq block.distinct_disc(4) block.exhaust_disc block_combine_add_simps(1) mem_Collect_eq par_blocks_exist_before)
+      subgoal by (smt (z3) c1.is_FREED'_eq c2.is_ALLOC'_eq c2.is_FREED'_eq block.exhaust_disc block_combine.simps(1) block_combine.simps(7) is_alloc_def) 
+      subgoal by (metis (no_types, lifting) c1.is_ALLOC'_eq c2.is_ALLOC'_eq block_combine.simps(7) is_alloc_def)
             
       done
           
     lemma is_FREED'_eq: "is_FREED s' b \<longleftrightarrow> b\<in>f\<^sub>1\<union>f\<^sub>2 \<or> is_FREED s b"  
       apply (auto simp: combine_states_def)
-      subgoal using c1.is_FREED'_eq c2.is_FREED'_eq cell_combine.elims by blast
-      subgoal by (metis (mono_tags, lifting) c1.is_FREED'_eq cell_combine_add_simps(2))
-      subgoal by (smt (verit) c2.is_FREED'_eq cell_combine_add_simps(3))
+      subgoal using c1.is_FREED'_eq c2.is_FREED'_eq block_combine.elims by blast
+      subgoal by (metis (mono_tags, lifting) c1.is_FREED'_eq block_combine_add_simps(2))
+      subgoal by (smt (verit) c2.is_FREED'_eq block_combine_add_simps(3))
       subgoal by (simp add: c2.valid_trans_imps(1))
       done
       
@@ -738,7 +771,7 @@ begin
       \<or> (is_valid_addr s\<^sub>2 a \<and> addr.block a \<notin> f\<^sub>1)"
       unfolding combine_states_def 
       apply clarsimp
-      by (smt (verit, del_insts) addr.case_eq_if block_size_noblock(3) c1.intf_consistent_loc_axioms c1.intf_f_freed c2.intf_consistent_loc_axioms c2.intf_f_freed cell.distinct(5) freed_blocks_def intf_consistent_loc.valid_block_trans is_block_def is_valid_addr_def mem_Collect_eq valid_block_trans_def zero_order(3))
+      by (smt (verit, del_insts) addr.case_eq_if block_size_noblock(3) c1.acc_consistent_loc_axioms c1.acc_f_freed c2.acc_consistent_loc_axioms c2.acc_f_freed block.distinct(5) freed_blocks_def acc_consistent_loc.valid_block_trans is_alloc_def is_valid_addr_def mem_Collect_eq valid_block_trans_def zero_order(3))
   
       
       
@@ -754,7 +787,7 @@ begin
       proof (cases "b \<in> a\<^sub>2")
         case True
         hence "is_FRESH s\<^sub>1 b"
-          by (smt (verit) alloc_blocks_def c1.intf_a_alloc c2.intf_a_alloc disjoint_iff feasible mem_Collect_eq spar_feasible_def)
+          by (smt (verit) alloc_blocks_def c1.acc_a_alloc c2.acc_a_alloc disjoint_iff feasible mem_Collect_eq spar_feasible_def)
         then show ?thesis
           using True
           by (auto simp add: combine_states_def get_addr_def)
@@ -769,10 +802,10 @@ begin
             apply (simp add: valid_addr')
             apply (simp add: is_valid_addr_alt)
             apply auto
-            by (metis True UnI1 Un_upper2 addr.sel(1) c1.valid_trans_imps(1) c2.intf_ref_not_fresh c2.is_FREED'_eq cell.exhaust_disc image_eqI subsetD)
+            by (metis True UnI1 Un_upper2 addr.sel(1) c1.valid_trans_imps(1) c2.acc_ref_not_fresh c2.is_FREED'_eq block.exhaust_disc image_eqI subsetD)
       
           have "is_ALLOC s b"
-            by (smt (verit, best) False \<open>is_ALLOC s\<^sub>2 b\<close> alloc_blocks_def c2.intf_a_alloc c2.valid_block_trans cell.exhaust_disc mem_Collect_eq valid_block_trans_def)
+            by (smt (verit, best) False \<open>is_ALLOC s\<^sub>2 b\<close> alloc_blocks_def c2.acc_a_alloc c2.valid_block_trans block.exhaust_disc mem_Collect_eq valid_block_trans_def)
 
           have A1: "is_ALLOC s\<^sub>1 b"
             by (smt (verit, best) ADDR \<open>is_ALLOC s b\<close> addr.case assms block_size_combine c1.valid_block_trans combine_states_def is_valid_addr_alt not_less_zero valid_block_trans_def)
@@ -780,7 +813,7 @@ begin
           show ?thesis using A1 A2
             apply (cases "mapp s\<^sub>1 b"; cases "mapp s\<^sub>2 b"; simp)
             apply (auto simp add: combine_states_def get_addr_def split: if_splits)
-            by (smt (verit, best) A1 A2 ADDR True addr.case assms block_size_def cell.simps(10) is_valid_addr_alt list_combine_inth mem_Collect_eq par_blocks_same_length)
+            by (smt (verit, best) A1 A2 ADDR True addr.case assms block_size_def block.simps(10) is_valid_addr_alt list_combine_inth mem_Collect_eq par_blocks_same_length)
           
         next
           case [simp]: False
@@ -794,7 +827,7 @@ begin
           next
             case False
             have A2: "is_ALLOC s\<^sub>2 b"
-              by (metis (no_types, lifting) ADDR False addr.case_eq_if addr.sel(1) assms cell.exhaust_disc combine_states_def is_valid_addr_alt valid_mcombine)
+              by (metis (no_types, lifting) ADDR False addr.case_eq_if addr.sel(1) assms block.exhaust_disc combine_states_def is_valid_addr_alt valid_mcombine)
 
             hence "is_ALLOC s b"
               by (simp add: c2.is_ALLOC'_eq)
@@ -810,7 +843,7 @@ begin
               
               apply (auto simp add: combine_states_def get_addr_def split: if_splits)
               apply (subst list_combine_inth)
-              subgoal by (metis block_size_def cell.disc(3) cell.simps(10) par_blocks_same_length)
+              subgoal by (metis block_size_def block.disc(3) block.simps(10) par_blocks_same_length)
               apply auto
               done
               
@@ -820,41 +853,41 @@ begin
     qed
             
     lemma get_addr1_orig: "\<lbrakk>is_valid_addr s a; is_valid_addr s' a; a \<notin> w\<^sub>1\<rbrakk> \<Longrightarrow> get_addr s\<^sub>1 a = get_addr s a"
-      using c1.intf_nw_untouched c1.valid_if_not_freed valid_addr' by blast
+      using c1.acc_nw_untouched c1.valid_if_not_freed valid_addr' by blast
       
     lemma get_addr2_orig: "\<lbrakk>is_valid_addr s a; is_valid_addr s' a; a \<notin> w\<^sub>2\<rbrakk> \<Longrightarrow> get_addr s\<^sub>2 a = get_addr s a"
-      using c2.addr_orig_val c2.intf_nw_untouched valid_addr' by blast
+      using c2.addr_orig_val c2.acc_nw_untouched valid_addr' by blast
       
     lemmas get_addr_orig = get_addr1_orig get_addr2_orig
       
-    lemma consistent': "intf_consistent s (i\<^sub>1+i\<^sub>2) s'"
-      unfolding intf_consistent_def Let_def split
+    lemma consistent': "acc_consistent s (i\<^sub>1+i\<^sub>2) s'"
+      unfolding acc_consistent_def Let_def split
       apply (intro conjI allI ballI)
       subgoal for b
-        using c1.intf_ref_not_fresh[of b] c2.intf_ref_not_fresh[of b]
+        using c1.acc_ref_not_fresh[of b] c2.acc_ref_not_fresh[of b]
         by (auto simp: is_FRESH'_eq)
       subgoal for b
-        using c1.intf_ref_not_freed[of b] c2.intf_ref_not_freed[of b]
+        using c1.acc_ref_not_freed[of b] c2.acc_ref_not_freed[of b]
         by (auto simp: )
       subgoal for a
         using c1.rw_valid_s c2.rw_valid_s by auto
       subgoal for a
         using c1.rw_valid_s' c2.rw_valid_s' apply (clarsimp simp: is_ALLOC'_eq)
-        by (metis Un_iff c1.intf_ref_not_fresh c1.is_ALLOC'_eq c1.is_FREED'_eq c2.intf_ref_not_fresh c2.is_ALLOC'_eq c2.is_FREED'_eq cell.disc(2) cell.exhaust_disc image_eqI valid_addr')
+        by (metis Un_iff c1.acc_ref_not_fresh c1.is_ALLOC'_eq c1.is_FREED'_eq c2.acc_ref_not_fresh c2.is_ALLOC'_eq c2.is_FREED'_eq block.disc(2) block.exhaust_disc image_eqI valid_addr')
       subgoal for b \<comment> \<open>Valid block trans\<close>
         using c1.valid_block_trans[of b] c2.valid_block_trans[of b]
         by (cases "mapp s\<^sub>1 b"; cases "mapp s\<^sub>2 b"; cases "mapp s b"; simp add: valid_block_trans_def combine_states_def)
       subgoal 
-        by (auto simp: c1.intf_a_alloc c2.intf_a_alloc alloc_blocks_def is_FRESH'_eq)
+        by (auto simp: c1.acc_a_alloc c2.acc_a_alloc alloc_blocks_def is_FRESH'_eq)
       subgoal        
-        by (auto simp: c1.intf_f_freed c2.intf_f_freed freed_blocks_def is_FREED'_eq)
+        by (auto simp: c1.acc_f_freed c2.acc_f_freed freed_blocks_def is_FREED'_eq)
         
       subgoal for a \<comment> \<open>Non-written addresses untouched\<close>
         by (auto simp: get_addr_combine get_addr_orig)
       done
         
     lemma alloc_block'_eq: "alloc_blocks s s' = alloc_blocks s s\<^sub>1 \<union> alloc_blocks s s\<^sub>2"
-      using c1.intf_a_alloc c2.intf_a_alloc consistent' intf_consistent_loc.intf_a_alloc intf_consistent_loc.intro intf_plus_simps(3) by blast
+      using c1.acc_a_alloc c2.acc_a_alloc consistent' acc_consistent_loc.acc_a_alloc acc_consistent_loc.intro acc_plus_simps(3) by blast
       
     lemma alloc_disj: "a\<^sub>1 \<inter> a\<^sub>2 = {}"
       using feasible spar_feasible_def by auto
@@ -885,23 +918,105 @@ begin
       using c1.freed_valid_s c2.valid_s_not_alloc
        by auto
       
+
+         
+    (* Stronger version of no-race as lemma, 
+      assuming acc_consistent + feasible!
+    *)  
+    lemma acc_norace_strong:
+      shows "acc_norace i\<^sub>1 i\<^sub>2 = (
+      let m\<^sub>1 = w\<^sub>1 \<union> {a. addr.block a \<in> a\<^sub>1 \<union> f\<^sub>1} in
+      let m\<^sub>2 = w\<^sub>2 \<union> {a. addr.block a \<in> a\<^sub>2 \<union> f\<^sub>2} in
+        (r\<^sub>1\<union>m\<^sub>1) \<inter> (m\<^sub>2) = {}
+      \<and> (m\<^sub>1) \<inter> (r\<^sub>2\<union>m\<^sub>2) = {})
+      "
+      apply (simp add: Let_def acc_norace_def set_eq_iff)
+      using alloc_addrs_approx_disj 
+      c1.a_dj_valid c2.rw_valid_or_alloc
+      c1.rw_valid_or_alloc c2.a_dj_valid
+      free_alloc_dj alloc_free_dj
+      by blast
+    
+    
+    
+    (* Properties of combine, for presentation in paper *)    
+    
+    lemma 
+    assumes "b \<in> a\<^sub>2\<union>f\<^sub>2"  
+    shows 
+      "is_FRESH s' b = is_FRESH s\<^sub>2 b" "is_FREED s' b = is_FREED s\<^sub>2 b" "is_ALLOC s' b = is_ALLOC s\<^sub>2 b"
+      using assms
+      apply (simp_all add: is_FRESH'_eq is_FREED'_eq is_ALLOC'_eq)
+      using c1.is_FRESH'_eq c2.is_FREED'_eq c2.is_FRESH'_eq assms apply blast
+      using c1.is_FREED'_eq c2.is_FREED'_eq free_alloc_dj apply blast
+      using c1.is_ALLOC'_eq c2.is_ALLOC'_eq free_alloc_dj assms apply blast
+      done
       
-      
+    lemma 
+    assumes "b \<notin> a\<^sub>2\<union>f\<^sub>2"  
+    shows 
+      "is_FRESH s' b = is_FRESH s\<^sub>1 b" "is_FREED s' b = is_FREED s\<^sub>1 b" "is_ALLOC s' b = is_ALLOC s\<^sub>1 b"
+      using assms
+      apply (simp_all add: is_FRESH'_eq is_FREED'_eq is_ALLOC'_eq)
+      using c1.is_FRESH'_eq c2.is_FREED'_eq c2.is_FRESH'_eq assms apply blast
+      using c1.is_FREED'_eq c2.is_FREED'_eq free_alloc_dj apply blast
+      using c1.is_ALLOC'_eq c2.is_ALLOC'_eq free_alloc_dj assms apply blast
+      done
+    
+    
+    lemma "is_FRESH s' b \<longleftrightarrow> (if b \<in> a\<^sub>2\<union>f\<^sub>2 then is_FRESH s\<^sub>2 b else is_FRESH s\<^sub>1 b)"
+      apply (simp add: is_FRESH'_eq)
+      using c1.is_FRESH'_eq c2.is_FREED'_eq c2.is_FRESH'_eq by blast
+    
+    lemma "is_FREED s' b \<longleftrightarrow> (if b \<in> a\<^sub>2\<union>f\<^sub>2 then is_FREED s\<^sub>2 b else is_FREED s\<^sub>1 b)"
+      apply (simp add: is_FREED'_eq)
+      using c1.is_FREED'_eq c2.is_FREED'_eq free_alloc_dj by auto
+    
+    lemma "is_ALLOC s' b \<longleftrightarrow> (if b \<in> a\<^sub>2\<union>f\<^sub>2 then is_ALLOC s\<^sub>2 b else is_ALLOC s\<^sub>1 b)"
+      apply (simp add: is_ALLOC'_eq)
+      using c1.is_ALLOC'_eq c2.is_ALLOC'_eq free_alloc_dj by auto
+
+    lemma 
+      fixes b i
+      defines "a \<equiv> ADDR b i"
+      assumes "is_ALLOC s' b" 
+      shows "get_addr s' a = (if a\<in>w\<^sub>2 \<or> b\<in>a\<^sub>2 \<or> b\<in>f\<^sub>2 then get_addr s\<^sub>2 a else get_addr s\<^sub>1 a)"  
+      apply (cases "is_valid_addr s' a")
+      subgoal
+        using assms(2)
+        by (auto simp: get_addr_combine a_def is_ALLOC'_eq)
+      subgoal
+        using assms(2)
+        apply (auto simp add: is_valid_addr_alt a_def get_addr_def)
+        apply (auto simp: block_size_def split: block.splits)
+        
+        subgoal
+          by (metis (no_types, lifting) UnI1 Un_commute addr.sel(1) addr.simps(2) assms(2) block_size_def c2.acc_consistent_loc_axioms c2.acc_ref_not_fresh c2.is_FREED'_eq block.simps(10) image_eqI acc_consistent_loc.rw_valid_s' is_ALLOC_conv is_FREED'_eq is_valid_addr_def valid_addr')
+        subgoal
+          by (smt (verit, ccfv_SIG) Un_iff alloc_blocks_def c1.acc_a_alloc c1.is_ALLOC'_eq c1.is_FRESH'_eq c2.acc_a_alloc c2.is_ALLOC'_eq block.disc(1) block.disc(2) block.disc(3) block.distinct(5) block.sel block_combine.simps(1) combine_states_def free_alloc_dj i_nth_simp(3) is_FREED'_eq le_eq_less_or_eq linorder_le_cases mapp_combine mem_Collect_eq par_blocks_exist_before)
+        subgoal 
+          by (meson UnI2 assms(2) is_ALLOC'_eq)
+        subgoal
+          by (metis Un_iff block_size_combine block_size_def c1.is_ALLOC'_eq c2.is_FREED'_eq block.collapse block.disc(3) block.distinct(5) block.simps(10) combine_states_def i_nth_simp(3) is_ALLOC'_eq is_FREED'_eq linorder_not_le)
+        done
+      done        
+    
   end
-  
+
+  text \<open>Consistent, feasible, and race free parallel executions\<close>  
   locale valid_parallel_execution =
     fixes s s\<^sub>1 i\<^sub>1 s\<^sub>2 i\<^sub>2
-    assumes c1[simp]: "intf_consistent s i\<^sub>1 s\<^sub>1"
-    assumes c2[simp]: "intf_consistent s i\<^sub>2 s\<^sub>2"
+    assumes c1[simp]: "acc_consistent s i\<^sub>1 s\<^sub>1"
+    assumes c2[simp]: "acc_consistent s i\<^sub>2 s\<^sub>2"
     assumes feasible: "spar_feasible i\<^sub>1 i\<^sub>2"
-    assumes norace: "intf_norace i\<^sub>1 i\<^sub>2"
+    assumes norace: "acc_norace i\<^sub>1 i\<^sub>2"
   begin  
 
     sublocale feasible_parallel_execution by (unfold_locales) (auto simp: feasible)
       
       
     lemma write_disjoint: "w\<^sub>1 \<inter> w\<^sub>2 = {}"
-      using norace unfolding intf_norace_def Let_def by auto
+      using norace unfolding acc_norace_def Let_def by auto
 
     
     subsection \<open>Symmetry\<close>  
@@ -917,7 +1032,7 @@ begin
           
           (* TODO: we break the abstraction barrier of get_addr twice! *)
           
-          obtain vs where [simp]: "mapp s b = BLOCK vs" 
+          obtain vs where [simp]: "mapp s b = ALLOC vs" 
             using par_blocks_exist_before[of b] 
             by (cases "mapp s b"; simp)
           
@@ -940,8 +1055,8 @@ begin
             
           
           show ?case
-            using write_disjoint c1.intf_nw_untouched[of "ADDR b _"]
-            using write_disjoint c2.intf_nw_untouched[of "ADDR b _"]
+            using write_disjoint c1.acc_nw_untouched[of "ADDR b _"]
+            using write_disjoint c2.acc_nw_untouched[of "ADDR b _"]
             apply (auto simp: list_eq_iff_nth_eq list_combine_nth eq_nat_nat_iff)
             by (metis int_nat_eq nat_int order_refl)
           
@@ -950,12 +1065,12 @@ begin
       
     lemma symmetric: "valid_parallel_execution s s\<^sub>2 i\<^sub>2 s\<^sub>1 i\<^sub>1"  
       apply unfold_locales
-      using feasible spar_feasible_sym intf_norace_sym norace
+      using feasible spar_feasible_sym acc_norace_sym norace
       by auto
       
       
     lemma freed_disj: "f\<^sub>1 \<inter> f\<^sub>2 = {}"  
-      using norace unfolding intf_norace_def Let_def
+      using norace unfolding acc_norace_def Let_def
       apply auto
       by (metis IntI UnI2 addr.sel(1) emptyE mem_Collect_eq)
       
@@ -977,10 +1092,10 @@ begin
       subgoal 
         by (simp add: c2.freed_addrs_def)
       subgoal 
-        by (smt Diff_iff UnE alloc_blocks_def c2.freed_addrs_def c2.is_FREED'_eq cell.distinct(2) disjoint_iff c1.intf_a_alloc c2.intf_a_alloc c1.valid_addrs'_subset mem_Collect_eq spar_feasible_def subsetD feasible)
+        by (smt Diff_iff UnE alloc_blocks_def c2.freed_addrs_def c2.is_FREED'_eq block.distinct(2) disjoint_iff c1.acc_a_alloc c2.acc_a_alloc c1.valid_addrs'_subset mem_Collect_eq spar_feasible_def subsetD feasible)
       subgoal by (simp add: addr.case_eq_if c1.is_ALLOC'_eq is_valid_addr_alt)
       subgoal 
-        by (smt Diff_iff UnE alloc_blocks_def c1.freed_addrs_def c1.is_FREED'_eq cell.distinct(2) disjoint_iff c1.intf_a_alloc c2.intf_a_alloc c2.valid_addrs'_subset mem_Collect_eq spar_feasible_def subsetD feasible)
+        by (smt Diff_iff UnE alloc_blocks_def c1.freed_addrs_def c1.is_FREED'_eq block.distinct(2) disjoint_iff c1.acc_a_alloc c2.acc_a_alloc c2.valid_addrs'_subset mem_Collect_eq spar_feasible_def subsetD feasible)
       subgoal using freed_disj by blast
       done
       
@@ -1002,109 +1117,5 @@ begin
             
                         
   end      
-  
-      
-    
-  (*  
-      
-      
-    
-  definition "valid_addr m a \<longleftrightarrow> cell.is_valid (mapp m a)"
-  
-  definition "m_fresh m \<equiv> {a. mapp m a = FRESH }"
-  definition "m_freed m \<equiv> {a. mapp m a = FREED }"
-  definition "m_valid m \<equiv> {a. cell.is_valid (mapp m a) }"
-    
-  lemma m_fresh_infinite[simp, intro!]: "infinite (m_fresh m)"
-    unfolding m_fresh_def
-    apply transfer
-    using finite_Collect_not infinite_UNIV by blast
-    
-    
-  datatype ('a,'idx) interference = interference (r: "('a\<times>'idx) set") (w: "('a\<times>'idx) set") (a: "'a set") (f: "'a set")
-  hide_const (open) r w a f  
-    
-  abbreviation "intf_r r \<equiv> interference r {} {} {}"
-  abbreviation "intf_w w \<equiv> interference {} w {} {}"
-  abbreviation "intf_a a \<equiv> interference {} {} a {}"
-  abbreviation "intf_f f \<equiv> interference {} {} {} f"
-
-  instantiation interference :: (type,type) comm_monoid_add
-  begin
-    definition "0 = interference {} {} {} {}"
-    definition "a+b \<equiv> case (a,b) of (interference ra wa aa fa, interference rb wb ab fb) \<Rightarrow>
-      interference (ra\<union>rb) (wa\<union>wb) (aa\<union>ab) (fa\<union>fb)"
-
-     instance
-       apply standard     
-       unfolding zero_interference_def plus_interference_def
-       by (auto split: interference.split)
-      
-  end
-  
-    
-  lemma interference_zero_simps[simp]:  
-    "interference.a 0 = {}"  
-    "interference.f 0 = {}"  
-    "interference.r 0 = {}"  
-    "interference.w 0 = {}"  
-    by (auto split: interference.split simp: zero_interference_def)
-    
-  lemma interference_plus_simps[simp]:
-    "interference.a (a+b) = interference.a a \<union> interference.a b"  
-    "interference.f (a+b) = interference.f a \<union> interference.f b"                     
-    "interference.r (a+b) = interference.r a \<union> interference.r b"  
-    "interference.w (a+b) = interference.w a \<union> interference.w b"  
-    by (auto split: interference.split simp: plus_interference_def)
-    
-  
-  text \<open>Over-approximation of everything that was modified: precise written addresses, and everything of allocated or freed blocks\<close>
-  definition "intf_modified i \<equiv> case i of (interference rd wr al fr) \<Rightarrow> wr \<union> (al\<union>fr)\<times>UNIV"
-    
-  definition "intf_compatible i\<^sub>1 i\<^sub>2 \<equiv> interference.a i\<^sub>1 \<inter> interference.a i\<^sub>2 = {}"
-  
-  definition "intf_nointer i\<^sub>1 i\<^sub>2 \<equiv> 
-    let m\<^sub>1 = intf_modified i\<^sub>1 in
-    let m\<^sub>2 = intf_modified i\<^sub>2 in
-    let r\<^sub>1 = interference.r i\<^sub>1 in
-    let r\<^sub>2 = interference.r i\<^sub>2 in
-      (r\<^sub>1 \<union> m\<^sub>1) \<inter> m\<^sub>2 = {}
-    \<and> m\<^sub>1 \<inter> (r\<^sub>2\<union>m\<^sub>2) = {}
-  "
-  
-  (*
-  definition "intf_nointer i\<^sub>1 i\<^sub>2 \<equiv> case (i\<^sub>1,i\<^sub>2) of (interference r\<^sub>1 w\<^sub>1 a\<^sub>1 f\<^sub>1, interference r\<^sub>2 w\<^sub>2 a\<^sub>2 f\<^sub>2) \<Rightarrow>
-    let ww\<^sub>1 = w\<^sub>1 \<union> a\<^sub>1 \<union> f\<^sub>1 in
-    let ww\<^sub>2 = w\<^sub>2 \<union> a\<^sub>2 \<union> f\<^sub>2 in
-      (r\<^sub>1 \<union> ww\<^sub>1) \<inter> ww\<^sub>2 = {}
-    \<and> ww\<^sub>1 \<inter> (r\<^sub>2\<union>ww\<^sub>2) = {}
-  "
-  *)
-   
-  definition "intf_consistent s i s' \<equiv> case i of (interference rd wr al fr) \<Rightarrow>
-    (finite (al\<union>fr))  
-  \<and> (\<forall>a\<in>-(wr\<union>al\<union>fr). mapp s a = mapp s' a)
-  \<and> (\<forall>a\<in>fr. mapp s a \<noteq> FREED \<and> mapp s' a = FREED)
-  \<and> (\<forall>a\<in>al. mapp s a = FRESH)
-  \<and> (\<forall>a\<in>(rd\<union>wr)-fr. cell.is_valid (mapp s' a))  
-  \<and> (\<forall>a\<in>(rd\<union>wr)-al. cell.is_valid (mapp s a))
-  "  
-
-  definition "combine_states s\<^sub>1 i\<^sub>2 s\<^sub>2 \<equiv> mcombine s\<^sub>1 (intf_modified i\<^sub>2) s\<^sub>2"
-
-  lemma intf_compatible_sym: "intf_compatible i\<^sub>1 i\<^sub>2 = intf_compatible i\<^sub>2 i\<^sub>1"  
-    by (auto simp: intf_compatible_def)
-
-  lemma intf_nointer_sym: "intf_nointer i\<^sub>1 i\<^sub>2 = intf_nointer i\<^sub>2 i\<^sub>1"  
-    by (auto simp: intf_nointer_def Let_def split: interference.split)
-  
-  lemma combine_states_sym: "intf_nointer i\<^sub>1 i\<^sub>2 \<Longrightarrow> intf_consistent s i\<^sub>1 s\<^sub>1 \<Longrightarrow> intf_consistent s i\<^sub>2 s\<^sub>2 \<Longrightarrow>
-    combine_states s\<^sub>1 i\<^sub>2 s\<^sub>2 = combine_states s\<^sub>2 i\<^sub>1 s\<^sub>1"
-    unfolding intf_nointer_def intf_consistent_def combine_states_def mext intf_modified_def
-    apply (auto split!: interference.splits simp: Let_def)
-    by (metis Compl_iff Un_iff boolean_algebra.de_Morgan_disj inter_compl_diff_conv)
-  
-  *)
-  
 
 end
