thys/examples/Par_Array_Examples.thy
@@ -1,0 +1,271 @@
+(** TODO: Maybe some nice parallel examples directly with VCG here?
+  currently, all more complex stuff is done via Sepref, and there's 
+  only the minimum required VCG setup!
+*)
+theory Par_Array_Examples
+imports "../sepref/IICF/Impl/IICF_Array"
+begin
+  declare [[llc_compile_par_call=true]]
+
+  context fixes f :: "'a \<Rightarrow> 'a" begin
+
+  fun abs_map where
+    "abs_map xs = (
+      if length xs \<le> 1 then map f xs 
+      else let
+        xs\<^sub>1 = take (length xs div 2) xs;
+        xs\<^sub>2 = drop (length xs div 2) xs;
+        xs\<^sub>1 = abs_map xs\<^sub>1;
+        xs\<^sub>2 = abs_map xs\<^sub>2
+      in
+        xs\<^sub>1@xs\<^sub>2
+      )"
+    
+    lemmas [simp del] = abs_map.simps  
+
+      
+    lemma "abs_map xs = map f xs"
+      apply (induction xs rule: abs_map.induct)
+      apply (subst abs_map.simps)
+      apply (auto split: if_splits)
+      by (metis atd_lem map_append)
+    
+    
+    definition "map1 \<equiv> RECT (\<lambda>map1 (xs,n). doN {
+      ASSERT (n = length xs);
+      if length xs = 0 then RETURN xs
+      else if length xs = 1 then doN {
+        x \<leftarrow> mop_list_get xs 0;
+        xs \<leftarrow> mop_list_set xs 0 (f x);
+        RETURN xs
+      } else doN {
+        let m = n div 2;
+        (_,xs) \<leftarrow> WITH_SPLIT m xs (\<lambda>xs\<^sub>1 xs\<^sub>2. do {
+          (xs\<^sub>1,xs\<^sub>2) \<leftarrow> nres_par map1 map1 (xs\<^sub>1,m) (xs\<^sub>2,n-m);
+          RETURN ((),(xs\<^sub>1,xs\<^sub>2))
+        });
+        RETURN xs
+      }
+      })"  
+      
+    schematic_goal map1_unfold: "map1 = ?foo"
+      unfolding map1_def
+      apply (subst RECT_unfold)
+      apply refine_mono
+      unfolding map1_def[symmetric]
+      ..
+      
+    lemma map_by_idx: "length xs = 1 \<Longrightarrow> xs[0:=f (xs!0)] = map f xs" by (cases xs) auto
+      
+    lemma aux1: "length xs\<^sub>1 = length (xs\<^sub>1 @ xs\<^sub>2) div 2 \<longleftrightarrow> length (xs\<^sub>1 @ xs\<^sub>2) div 2 = length xs\<^sub>1" by auto
+    
+    lemma "n=length xs \<Longrightarrow> map1 (xs,n) \<le> RETURN (map f xs)"  
+      unfolding map1_def  
+      apply (refine_vcg RECT_rule[where V="measure snd" and pre="\<lambda>(xs,n). n=length xs" and M="\<lambda>(xs,n). RETURN (map f xs)", THEN order_trans])
+      apply simp
+      apply simp
+      apply simp
+      apply simp
+      apply simp
+      apply simp
+      apply (simp add: map_by_idx)
+      apply simp
+      
+      apply (simp only: split prod.inject, elim conjE)
+      apply (thin_tac "length a = length a" for a)
+      apply (thin_tac "RECT _ = _")
+      apply hypsubst
+      apply (simp only: aux1)
+      
+      apply (rule order_trans, rprems)
+      apply simp_all
+      apply auto []
+      apply (rule order_trans, rprems)
+      apply auto
+      by (metis div2_Suc_Suc length_0_conv nat.distinct(1) old.nat.exhaust)
+    
+    
+    
+    oops
+    proof (induction xs arbitrary: n rule: abs_map.induct)
+      case (1 xs)
+      
+      note IH1="1"(1)[of _ _ "length xs div 2", OF _ _ refl]
+      
+      note [simp] = \<open>n=length xs\<close>
+      
+      have aux1: "(xs,n) = (a,b) \<longleftrightarrow> a=xs \<and> b=n" for a b by auto
+      
+      show ?case
+        apply (subst map1_unfold)
+        apply (subst abs_map.simps)
+        unfolding WITH_SPLIT_def
+        apply refine_vcg
+        apply simp
+        apply simp
+        apply simp
+        apply simp
+        apply simp
+        apply (cases xs; simp)
+        apply simp
+        apply (subst (asm) aux1, elim conjE)
+        apply (simp only:, hypsubst)
+        apply (rule order_trans[OF IH1])
+        apply simp
+        apply simp
+        apply simp
+        apply refine_vcg
+        
+      
+      
+      
+    qed
+      
+      
+      
+          
+  end  
+
+    
+    
+  context
+    includes monad_syntax_M
+  begin
+  
+  definition par_incr :: "8 word ptr \<times> 64 word \<Rightarrow> 8 word ptr llM"
+  where [llvm_code]: "par_incr \<equiv> MMonad.REC (\<lambda>par_incr (p,n).
+    if n=1 then doM {
+      x \<leftarrow> array_nth p (0::64 word);
+      x \<leftarrow> ll_udiv x 2;
+      array_upd p (0::64 word) x;
+      return p
+    } else doM {
+      i \<leftarrow> ll_sdiv n 2;
+      (p\<^sub>1,p\<^sub>2) \<leftarrow> ars_split i p;
+      llc_par par_incr par_incr (p\<^sub>1,i) (p\<^sub>2,n-i);
+      ars_join p\<^sub>1 p\<^sub>2;
+      return p
+    })"
+  
+  end  
+  
+  export_llvm par_incr
+  
+  schematic_goal par_incr_unfold: "par_incr = ?foo"
+    unfolding par_incr_def
+    apply (subst MMonad.REC_unfold)
+    apply pf_mono_prover
+    unfolding par_incr_def[symmetric]
+    ..
+  
+    
+  lemma "llvm_htriple 
+    (raw_array_slice_assn xs xsi ** snat_assn n ni ** \<up>(n=length xs)) 
+    (par_incr (xsi,ni))
+    (\<lambda>_. raw_array_slice_assn (abs_map (\<lambda>x. x div 2) xs) xsi)
+    "
+  proof (induction xs rule: abs_map.induct[where f="(\<lambda>x. x div 2)"])
+    case (1 xs)
+    show ?case
+      apply (subst par_incr_unfold)
+      apply (rule htriple_pure_preI, ((determ \<open>drule pure_part_split_conj|erule conjE\<close>)+)?)
+      apply vcg_monadify
+      
+      find_theorems pure_part LLVM_DS_NArray.array_slice_assn
+      
+      apply vcg
+      apply vcg_rl
+      apply vcg_try_solve
+    
+    
+  qed
+    
+    
+    unfolding par_incr_def
+    apply (rule REC_rule[where V="measure nat" and P="\<lambda>t ()"])
+    apply vcg
+    apply pf_mono_prover
+  
+  
+  
+  
+  
+  
+  
+  
+  lemma REC_rule: (* Needs annotation to be usable in automated setting! *)
+    assumes WF: "wf V"
+    assumes MONO: "M_mono_body B"
+    assumes STEP: "\<And>D t x. \<lbrakk>\<And>t' x. (t',t)\<in>V \<Longrightarrow> htriple (P t' x ** F) (D x) (Q x) \<rbrakk> \<Longrightarrow> htriple (P t x ** F) (B D x) (Q x)"
+    assumes INIT: "P' \<turnstile> P t x ** F"
+    shows "htriple P' (MMonad.REC B x) (Q x)"
+  proof -  
+  
+    have "htriple (P t x ** F) (MMonad.REC B x) (Q x)"
+      using WF
+      apply (induction t arbitrary: x)
+      apply (subst MMonad.REC_unfold[OF MONO])
+      by (rule STEP)
+    thus ?thesis
+      apply (rule cons_rule)
+      subgoal using INIT unfolding entails_def by simp
+      subgoal .
+      .
+  qed
+
+
+
+  declare [[llc_compile_par_call=true]]
+
+  find_theorems raw_array_slice_assn
+
+  context
+    includes monad_syntax_M
+  begin
+
+  definition [llvm_code]: ""
+  
+  
+  
+  definition [llvm_code]: "par_incr (p::8 word ptr) (n::64 word) \<equiv> MMonad.REC (\<lambda>par_incr (p,n).
+    if n=1 then doM {
+      x \<leftarrow> array_nth p (0::64 word);
+      x \<leftarrow> ll_udiv x 2;
+      array_upd p (0::64 word) x;
+      return p
+    } else doM {
+      i \<leftarrow> ll_sdiv n 2;
+      (p\<^sub>1,p\<^sub>2) \<leftarrow> ars_split i p;
+      llc_par par_incr par_incr (p\<^sub>1,i) (p\<^sub>2,n-i);
+      ars_join p\<^sub>1 p\<^sub>2;
+      return p
+    }) (p,n)
+  "
+
+  
+  export_llvm par_incr
+  
+  lemma
+    shows ""
+  
+  
+  
+  lemma "llvm_htriple 
+    (raw_array_slice_assn xs xsi ** snat_assn n ni ** \<up>(n=length xs)) 
+    (par_incr xsi ni)
+    (\<lambda>_. raw_array_slice_assn (map (\<lambda>x. x div 2) xs) xsi)
+    "
+    unfolding par_incr_def
+    apply (rule REC_rule[where V="measure nat" and P="\<lambda>t ()"])
+    apply vcg
+    apply pf_mono_prover
+    
+  
+    find_theorems MMonad.REC 
+    
+  
+  end
+
+
+
+end
